spot/GC.SPOT.HeapExpansion.fst
@@ -1958,6 +1958,34 @@ let spot_chunked_promote_object_head_split_preserves_old_non_blue_header
   CheneyPreservation.chunked_promote_object_head_split_preserves_old_non_blue_header
     minor mh obj fp wosize fuel src hdr
 
+let spot_chunked_promote_object_head_split_preserves_old_non_blue_field
+  (minor: minor_state) (mh: MH.major_heap) (obj: U64.t)
+  (fp: U64.t) (wosize: nat{wosize > 0}) (fuel: nat)
+  (src: obj_addr) (hdr: U64.t) (j: nat) (field_addr: hp_addr)
+  (old: U64.t)
+  : Lemma
+      (requires
+        fuel > 1 /\
+        fp <> 0UL /\
+        GenInv.chunked_major_alloc_shape mh fp fuel /\
+        SpecMajorAlloc.major_fl_chain_terminates mh fp fuel = true /\
+        GenInv.chunked_chain_objects_blue mh fp fuel /\
+        SpecMajorAlloc.major_fl_head_wosize mh fp >= wosize + 2 /\
+        Seq.mem src (MH.major_objects mh) /\
+        MH.read_word_in_major mh (hd_address src) == Some hdr /\
+        Obj.getColor hdr <> GC.Lib.Header.Blue /\
+        j < U64.v (Obj.getWosize hdr) /\
+        U64.v field_addr == U64.v src + j * U64.v mword /\
+        MH.read_word_in_major mh field_addr == Some old)
+      (ensures
+        (let res =
+           ChunkedPromote.chunked_promote_object_with_fuel
+             minor mh obj fp wosize fuel in
+         MH.read_word_in_major res.major_out field_addr == Some old))
+  =
+  CheneyPreservation.chunked_promote_object_head_split_preserves_old_non_blue_field
+    minor mh obj fp wosize fuel src hdr j field_addr old
+
 let spot_chunked_promote_object_head_split_preserves_remaining_head_wosize
   (minor: minor_state) (mh: MH.major_heap) (obj: U64.t)
   (fp: U64.t) (wosize: nat{wosize > 0}) (fuel: nat)
